src/ocaml/extraction/SSA2QFBV.ml
@@ -711,6 +711,33 @@ let qfbv_spec_algsnd_la s =
   qfbv_spec_algsnd_la_rec (bexp_rbexp (SSA.SSA.rspre s))
     (bexp_program_algsnd_split_fixed_final fE (SSA.SSA.rsprog s))
 
+(** val make_sndcond :
+    TypEnv.SSATE.env -> SSA.SSA.rbexp -> SSA.SSA.instr list -> SSA.SSA.instr
+    -> QFBV.QFBV.bexp **)
+
+let make_sndcond fE f p i =
+  let ef = bexp_rbexp f in
+  let vs = SSA.SSA.depvars_rpre_rprogram (SSA.SSA.rvs_instr i) f p in
+  let ep = bexp_program fE (SSA.SSA.slice_rprogram vs p) in
+  let es = bexp_instr_algsnd fE i in
+  QFBV.QFBV.qfbv_imp (QFBV.QFBV.qfbv_conj ef (QFBV.QFBV.qfbv_conjs_la ep)) es
+
+(** val algsnd_slice_la_rec :
+    TypEnv.SSATE.env -> SSA.SSA.program -> SSA.SSA.rbexp -> SSA.SSA.program
+    -> QFBV.QFBV.bexp list **)
+
+let rec algsnd_slice_la_rec fE pre f = function
+| [] -> []
+| hd :: tl ->
+  (make_sndcond fE f pre hd) :: (algsnd_slice_la_rec fE (rcons pre hd) f tl)
+
+(** val algsnd_slice_la : SSA.SSA.rspec -> QFBV.QFBV.bexp list **)
+
+let algsnd_slice_la s =
+  let fE = SSA.SSA.program_succ_typenv (SSA.SSA.rsprog s) (SSA.SSA.rsinputs s)
+  in
+  algsnd_slice_la_rec fE [] (SSA.SSA.rspre s) (SSA.SSA.rsprog s)
+
 (** val rngred_algsnd_split_la : SSA.SSA.rspec -> QFBV.QFBV.bexp list **)
 
 let rngred_algsnd_split_la s =
@@ -720,4 +747,4 @@ let rngred_algsnd_split_la s =
     SSA.SSA.rspec -> QFBV.QFBV.bexp list **)
 
 let rngred_algsnd_slice_split_la s =
-  cat (rngred_rspec_slice_split_la s) (qfbv_spec_algsnd_la s)
+  cat (rngred_rspec_slice_split_la s) (algsnd_slice_la s)
